---
id: "doe-rise-vase"
created: "Tue Dec 21 12:29:57 2021"
global_id: "lbroLt"
---

These equations describe the BÃ©zier curve $x(t)$ and $y(t)$ functions on the domain $0 \leq t \leq 1$:

$$x(t) = (1-t)^3\, x_1 + 3(1-t)^2 t\, x_2 + 3(1-t) t^2\, x_3 + t^3\, x_4$$
and
$$y(t) = (1-t)^3\, y_1 + 3(1-t)^2 t\, y_2 + 3(1-t) t^2\, y_3 + t^3\, y_4$$

A. Cross out the terms that go to zero at $t=0$ and show that this ensures that $x(t=0) = x_1$ and $y(t=0) = y_1$. 

B. Similarly, Cross out the terms that go to zero at $t=1$ and show that this ensures that $x(t=1) = x_4$ and $y(t=1) = y_4$.

